# Aufgabe 15
## 1)
$\chi_A(t)=\begin{vmatrix}t-5&2&-2&-8\\-6&t+2&-2&-8\\0&0&t&-1\\0&0&0&t+1\end{vmatrix}=(t+1)\cdot t\cdot \begin{vmatrix}t-5&2\\-6&t+2\end{vmatrix}=(t^2-t)\cdot((t-5)(t+2)+12)=t(t-1)(t^2-3t+2)=t(t+1)(t-2)(t-1)$

$\implies\sigma(A)=\{-1,0,1,2\}$

$V_{-1}=Ker(A+I)=Ker(\begin{pmatrix}6&-2&2&8\\6&-1&2&8\\0&0&1&1\\0&0&0&0\end{pmatrix})=Ker(\begin{pmatrix}1&0&0&1\\0&1&0&0\\0&0&1&1\\0&0&0&0\end{pmatrix})=\langle\begin{pmatrix}-1\\0\\-1\\1\end{pmatrix}\rangle_\Complex$

$V_0=Ker(A-0I)=Ker(\begin{pmatrix}5&-2&2&8\\6&-2&2&8\\0&0&0&1\\0&0&0&-1\end{pmatrix})=Ker(\begin{pmatrix}1&0&0&0\\0&1&-1&0\\0&0&0&0\\0&0&0&1\end{pmatrix})=\langle\begin{pmatrix}0\\1\\1\\0\end{pmatrix}\rangle_\Complex$

$V_1=Ker(A-1I)=Ker(\begin{pmatrix}4&-2&2&8\\6&-3&2&8\\0&0&-1&1\\0&0&0&-2\end{pmatrix})=Ker(\begin{pmatrix}0&0&0&0\\2&-1&0&0\\0&0&1&0\\0&0&0&1\end{pmatrix})=\langle\begin{pmatrix}1\\2\\0\\0\end{pmatrix}\rangle_\Complex$

$V_2=Ker(A-2I)=Ker(\begin{pmatrix}3&-2&2&8\\6&-4&2&8\\0&0&-2&1\\0&0&0&-3\end{pmatrix})=Ker(\begin{pmatrix}0&0&0&0\\3&-2&0&0\\0&0&1&0\\0&0&0&1\end{pmatrix})=\langle\begin{pmatrix}2\\3\\0\\0\end{pmatrix}\rangle_\Complex$

## 2)
-1 0 1 2

$J=\begin{pmatrix}-1&0&0&0\\0&0&0&0\\0&0&1&0\\0&0&0&2\end{pmatrix}$
$S=\begin{pmatrix}-1&0&1&2\\0&1&2&3\\-1&1&0&0\\1&0&0&0\end{pmatrix}$

$\begin{pmatrix}-1&0&1&2&1&0&0&0\\0&1&2&3&0&1&0&0\\-1&1&0&0&0&0&1&0\\1&0&0&0&0&0&0&1\end{pmatrix}$ -I,III+I,IV-I

$\begin{pmatrix}1&0&-1&-2&-1&0&0&0\\0&1&2&3&0&1&0&0\\0&1&-1&-2&-1&0&1&0\\0&0&1&2&1&0&0&1\end{pmatrix}$ III-II

$\begin{pmatrix}1&0&-1&-2&-1&0&0&0\\0&1&2&3&0&1&0&0\\0&0&-3&-5&-1&-1&1&0\\0&0&1&2&1&0&0&1\end{pmatrix}$ -III,III-2IV

$\begin{pmatrix}1&0&-1&-2&-1&0&0&0\\0&1&2&3&0&1&0&0\\0&0&1&1&-1&1&-1&-2\\0&0&1&2&1&0&0&1\end{pmatrix}$ I+III,II-2III,IV-III

$\begin{pmatrix}1&0&0&-1&-2&1&-1&-2\\0&1&0&1&2&-1&2&4\\0&0&1&1&-1&1&-1&-2\\0&0&0&1&2&-1&1&3\end{pmatrix}$ I+IV,II-IV,III-IV

$\begin{pmatrix}1&0&0&0&0&0&0&1\\0&1&0&0&0&0&1&1\\0&0&1&0&-3&2&-2&-5\\0&0&0&1&2&-1&1&3\end{pmatrix}$

$\implies S^{-1}=\begin{pmatrix}0&0&0&1\\0&0&1&1\\-3&2&-2&-5\\2&-1&1&3\end{pmatrix}$

$\exp(A)=S\exp(J)S^{-1}=\begin{pmatrix}-1&0&1&2\\0&1&2&3\\-1&1&0&0\\1&0&0&0\end{pmatrix}\cdot\begin{pmatrix}\frac1e&0&0&0\\0&1&0&0\\0&0&e&0\\0&0&0&e^2\end{pmatrix}\cdot\begin{pmatrix}0&0&0&1\\0&0&1&1\\-3&2&-2&-5\\2&-1&1&3\end{pmatrix}$

$=\begin{pmatrix}-\frac1e&0&e&2e^2\\0&1&2e&3e^2\\-\frac1e&1&0&0\\\frac1e&0&0&0\end{pmatrix}\cdot\begin{pmatrix}0&0&0&1\\0&0&1&1\\-3&2&-2&-5\\2&-1&1&3\end{pmatrix}=\begin{pmatrix}4e^2-3e&-2e^2+2e&2e^2-2e&\frac{6e^3-5e-1}{e}\\6e^2-6e&-3e^2+4e&3e^2-4e+1&9e^2-10e+1\\0&0&1&\frac{-1+e}{e}\\0&0&0&\frac1e\end{pmatrix}$

# Aufgabe 16
$A=\begin{pmatrix}4&-3\\2&-1\end{pmatrix}$

$\chi_A(t)=t^2-3t+2=(t-1)(t-2)$
$\sigma(A)=\{1,2\}$

$V_1=Ker(A-I)=Ker(\begin{pmatrix}3&-3\\2&-2\end{pmatrix})=Ker(\begin{pmatrix}1&-1\\0&0\end{pmatrix})=\langle\begin{pmatrix}1\\1\end{pmatrix}\rangle$

$V_2=Ker(A-2I)=Ker(\begin{pmatrix}2&-3\\2&-3\end{pmatrix})=Ker(\begin{pmatrix}2&-3\\0&0\end{pmatrix})=\langle\begin{pmatrix}3\\2\end{pmatrix}\rangle$

$J=\begin{pmatrix}1&0\\0&2\end{pmatrix}$
$S=\begin{pmatrix}1&3\\1&2\end{pmatrix},S^{-1}=\frac1{Det(S)}\begin{pmatrix}2&-3\\-1&1\end{pmatrix}=\begin{pmatrix}-2&3\\1&-1\end{pmatrix}$

$\begin{pmatrix}x_1(t)\\x_2(t)\end{pmatrix}=S\exp(tJ)S^{-1}\begin{pmatrix}2\\1\end{pmatrix}=\begin{pmatrix}1&3\\1&2\end{pmatrix}\begin{pmatrix}e^t&0\\0&e^{2t}\end{pmatrix}\begin{pmatrix}-2&3\\1&-1\end{pmatrix}\begin{pmatrix}2\\1\end{pmatrix}$

$=\begin{pmatrix}1&3\\1&2\end{pmatrix}\begin{pmatrix}e^t&0\\0&e^{2t}\end{pmatrix}\begin{pmatrix}-1\\1\end{pmatrix}=\begin{pmatrix}1&3\\1&2\end{pmatrix}\begin{pmatrix}-e^t\\e^{2t}\end{pmatrix}=\begin{pmatrix}3e^{2t}-e^t\\2e^{2t}-e^t\end{pmatrix}$